src/StructuredEncryption/runtimes/net/Generated/EncryptStructureInput.cs
@@ -6,6 +6,10 @@ using System;
  public class EncryptStructureInput {
  private AWS.Cryptography.StructuredEncryption.StructuredData _plaintextStructure ;
  private AWS.Cryptography.StructuredEncryption.CryptoSchema _cryptoSchema ;
+ private AWS.Cryptography.MaterialProviders.IKeyring _keyring ;
+ private AWS.Cryptography.MaterialProviders.ICryptographicMaterialsManager _cmm ;
+ private System.Collections.Generic.Dictionary<string, string> _implicitEncryptionContext ;
+ private System.Collections.Generic.Dictionary<string, string> _explicitEncryptionContext ;
  public AWS.Cryptography.StructuredEncryption.StructuredData PlaintextStructure {
  get { return this._plaintextStructure; }
  set { this._plaintextStructure = value; }
@@ -19,6 +23,34 @@ using System;
 }
  internal bool IsSetCryptoSchema () {
  return this._cryptoSchema != null;
+}
+ public AWS.Cryptography.MaterialProviders.IKeyring Keyring {
+ get { return this._keyring; }
+ set { this._keyring = value; }
+}
+ internal bool IsSetKeyring () {
+ return this._keyring != null;
+}
+ public AWS.Cryptography.MaterialProviders.ICryptographicMaterialsManager Cmm {
+ get { return this._cmm; }
+ set { this._cmm = value; }
+}
+ internal bool IsSetCmm () {
+ return this._cmm != null;
+}
+ public System.Collections.Generic.Dictionary<string, string> ImplicitEncryptionContext {
+ get { return this._implicitEncryptionContext; }
+ set { this._implicitEncryptionContext = value; }
+}
+ internal bool IsSetImplicitEncryptionContext () {
+ return this._implicitEncryptionContext != null;
+}
+ public System.Collections.Generic.Dictionary<string, string> ExplicitEncryptionContext {
+ get { return this._explicitEncryptionContext; }
+ set { this._explicitEncryptionContext = value; }
+}
+ internal bool IsSetExplicitEncryptionContext () {
+ return this._explicitEncryptionContext != null;
 }
  public void Validate() {
  if (!IsSetPlaintextStructure()) throw new System.ArgumentException("Missing value for required property 'PlaintextStructure'");
