src/StructuredEncryption/src/StructuredEncryptionClient.dfy
@@ -1,14 +1,13 @@
-include "../../StandardLibrary/StandardLibrary.dfy"
-include "../../StandardLibrary/UInt.dfy"
-include "../model/AwsCryptographyStructuredEncryptionTypes.dfy"
+include "../../../private-aws-encryption-sdk-dafny-staging/src/StandardLibrary/StandardLibrary.dfy"
+// TODO including UInt in this file causes build issues. It complains of duplicate UInt modules...
+include "../Model/AwsCryptographyStructuredEncryptionTypes.dfy"
 
 module {:extern "Dafny.Aws.StructuredEncryption.StructuredEncryptionClient"} StructuredEncryptionClient {
   import opened Wrappers
-  import opened UInt = StandardLibrary.UInt
   import opened StandardLibrary
-  import opened AwsCryptographyStructuredEncryptionTypes
+  import Types = AwsCryptographyStructuredEncryptionTypes
 
-  class StructuredEncryptionClient extends IStructuredEncryptionClient {
+  class StructuredEncryptionClient extends Types.IStructuredEncryptionClient {
     predicate ValidState()
     ensures ValidState() ==> History in Modifies
     {
@@ -18,47 +17,55 @@ module {:extern "Dafny.Aws.StructuredEncryption.StructuredEncryptionClient"} Str
     constructor()
       ensures ValidState() && fresh(Modifies) && fresh(History)
     {
-      History := new IStructuredEncryptionClientCallHistory();
+      History := new Types.IStructuredEncryptionClientCallHistory();
       Modifies := {History};
     }
 
     predicate EncryptStructureEnsuresPublicly(
-      input: EncryptStructureInput, 
-      output: Result<EncryptStructureOutput, Error>)
+      input: Types.EncryptStructureInput, 
+      output: Result<Types.EncryptStructureOutput, Types.Error>)
     {
       true
     }
 
     predicate DecryptStructureEnsuresPublicly(
-      input: DecryptStructureInput, 
-      output: Result<DecryptStructureOutput, Error>)
+      input: Types.DecryptStructureInput, 
+      output: Result<Types.DecryptStructureOutput, Types.Error>)
     {
       true
     }
 
-    method EncryptStructure(input: EncryptStructureInput)
-        returns (output: Result<EncryptStructureOutput, Error>)
+    method EncryptStructure(input: Types.EncryptStructureInput)
+        returns (output: Result<Types.EncryptStructureOutput, Types.Error>)
       requires ValidState()
       modifies Modifies - {History},
         History`EncryptStructure
       ensures EncryptStructureEnsuresPublicly(input, output)
-      ensures History.EncryptStructure == old(History.EncryptStructure) + [DafnyCallEvent(input, output)]
+      ensures History.EncryptStructure == old(History.EncryptStructure) + [Types.DafnyCallEvent(input, output)]
     {
+      // Ensure a Keyring XOR a CMM was included on input, otherwise error
+      :- Need(input.cmm.Some? || input.keyring.Some?,
+        Types.Error.StructuredEncryptionException(
+          message := "Invalid input: A Keyring or CMM MUST be supplied on input."));
+      :- Need(input.cmm.None? || input.keyring.None?,
+        Types.Error.StructuredEncryptionException(
+          message := "Invalid input: Cannot recieve both a Keyring and a CMM on input."));
+
       // TODO: Currently stubbed out to return a hardcoded StructuredData
       var stubbedBytes := [0x21, 0x64, 0x6c, 0x72, 0x6f, 0x77, 0x20, 0x2c, 0x6f, 0x6c, 0x6c, 0x65, 0x68];
-      var stubbedStructure := StructuredData(
-        content := StructuredDataContent.dataMap(
+      var stubbedStructure := Types.StructuredData(
+        content := Types.StructuredDataContent.dataMap(
           StructuredDataMap := map[
-            "foo" := StructuredData(
-              content := StructuredDataContent.terminal(Terminal:=stubbedBytes),
+            "foo" := Types.StructuredData(
+              content := Types.StructuredDataContent.terminal(Terminal:=stubbedBytes),
               attributes := None()
             ),
-            "bar" := StructuredData(
-              content := StructuredDataContent.terminal(Terminal:=stubbedBytes),
+            "bar" := Types.StructuredData(
+              content := Types.StructuredDataContent.terminal(Terminal:=stubbedBytes),
               attributes := None()
             ),
-            "fizzbuzz" := StructuredData(
-              content := StructuredDataContent.terminal(Terminal:=stubbedBytes),
+            "fizzbuzz" := Types.StructuredData(
+              content := Types.StructuredDataContent.terminal(Terminal:=stubbedBytes),
               attributes := None()
             )
           ]
@@ -66,35 +73,48 @@ module {:extern "Dafny.Aws.StructuredEncryption.StructuredEncryptionClient"} Str
         attributes := None()
       );
 
-      var encryptOutput := EncryptStructureOutput(ciphertextStructure := stubbedStructure);
+      var encryptOutput := Types.EncryptStructureOutput(ciphertextStructure := stubbedStructure);
 
       output := Success(encryptOutput);
-      History.EncryptStructure := History.EncryptStructure + [DafnyCallEvent(input, output)];
+      History.EncryptStructure := History.EncryptStructure + [Types.DafnyCallEvent(input, output)];
     }
     
-    method DecryptStructure(input: DecryptStructureInput)
-        returns (output: Result<DecryptStructureOutput, Error>)
+    method DecryptStructure(input: Types.DecryptStructureInput)
+        returns (output: Result<Types.DecryptStructureOutput, Types.Error>)
       requires ValidState()
       modifies Modifies - {History},
         History`DecryptStructure
       ensures DecryptStructureEnsuresPublicly(input, output)
-      ensures History.DecryptStructure == old(History.DecryptStructure) + [DafnyCallEvent(input, output)]
+      ensures History.DecryptStructure == old(History.DecryptStructure) + [Types.DafnyCallEvent(input, output)]
     {
+      // Ensure a Keyring XOR a CMM was included on input, otherwise error
+      :- Need(input.cmm.Some? || input.keyring.Some?,
+        Types.Error.StructuredEncryptionException(
+          message := "Invalid input: A Keyring or CMM MUST be supplied on input."));
+      :- Need(input.cmm.None? || input.keyring.None?,
+        Types.Error.StructuredEncryptionException(
+          message := "Invalid input: Cannot recieve both a Keyring and a CMM on input."));
+
+      // Ensure CryptoSchemas is not empty
+      :- Need(|input.cryptoSchemas| > 0,
+        Types.Error.StructuredEncryptionException(
+          message := "Invalid input: a non-empty Crypto Schema map must be supplied on input."));
+
       // TODO: Currently stubbed out to return a hardcoded StructuredData
       var stubbedBytes := [0x68, 0x65, 0x6c, 0x6c, 0x6f, 0x2c, 0x20, 0x77, 0x6f, 0x72, 0x6c, 0x64];
-      var stubbedStructure := StructuredData(
-        content := StructuredDataContent.dataMap(
+      var stubbedStructure := Types.StructuredData(
+        content := Types.StructuredDataContent.dataMap(
           StructuredDataMap := map[
-            "foo" := StructuredData(
-              content := StructuredDataContent.terminal(Terminal:=stubbedBytes),
+            "foo" := Types.StructuredData(
+              content := Types.StructuredDataContent.terminal(Terminal:=stubbedBytes),
               attributes := None()
             ),
-            "bar" := StructuredData(
-              content := StructuredDataContent.terminal(Terminal:=stubbedBytes),
+            "bar" := Types.StructuredData(
+              content := Types.StructuredDataContent.terminal(Terminal:=stubbedBytes),
               attributes := None()
             ),
-            "fizzbuzz" := StructuredData(
-              content := StructuredDataContent.terminal(Terminal:=stubbedBytes),
+            "fizzbuzz" := Types.StructuredData(
+              content := Types.StructuredDataContent.terminal(Terminal:=stubbedBytes),
               attributes := None()
             )
           ]
@@ -102,9 +122,9 @@ module {:extern "Dafny.Aws.StructuredEncryption.StructuredEncryptionClient"} Str
         attributes := None()
       );
 
-      var decryptOutput := DecryptStructureOutput(plaintextStructure := stubbedStructure);
+      var decryptOutput := Types.DecryptStructureOutput(plaintextStructure := stubbedStructure);
       output := Success(decryptOutput);
-      History.DecryptStructure := History.DecryptStructure + [DafnyCallEvent(input, output)];
+      History.DecryptStructure := History.DecryptStructure + [Types.DafnyCallEvent(input, output)];
     }
   }
 }
