src/StructuredEncryption/test/HappyCaseTests.dfy
@@ -1,17 +1,33 @@
-include "../../StandardLibrary/StandardLibrary.dfy"
-include "../../StandardLibrary/UInt.dfy"
+include "../../../private-aws-encryption-sdk-dafny-staging/src/StandardLibrary/StandardLibrary.dfy"
 include "../src/StructuredEncryptionClient.dfy"
-include "../model/AwsCryptographyStructuredEncryptionTypes.dfy"
+include "../Model/AwsCryptographyStructuredEncryptionTypes.dfy"
+include "../../../private-aws-encryption-sdk-dafny-staging/src/AwsCryptographicMaterialProviders/src/Index.dfy"
 
 module HappyCaseTests {
   import opened Wrappers
-  import opened UInt = StandardLibrary.UInt
   import opened StandardLibrary
   import opened AwsCryptographyStructuredEncryptionTypes
   import StructuredEncryptionClient
+  import AwsCryptographyMaterialProvidersTypes
+  import MaterialProviders
 
   method {:test} TestEncryptStructure() {
     var client := new StructuredEncryptionClient.StructuredEncryptionClient();
+
+    // Create keyring. Currently doesn't matter what keyring we create.
+    var matProvRes := MaterialProviders.MaterialProviders(MaterialProviders.DefaultMaterialProvidersConfig());
+    expect matProvRes.Success?;
+    var matProv := matProvRes.value;
+
+    var keyringInput := AwsCryptographyMaterialProvidersTypes.CreateAwsKmsMrkMultiKeyringInput(
+        generator := Some("arn:aws:kms:us-west-2:658956600833:key/b3537ef1-d8dc-4780-9f5a-55776cbb2f7f"),
+        kmsKeyIds := None(),
+        clientSupplier := None(),
+        grantTokens := None()
+    );
+    var keyringRes := matProv.CreateAwsKmsMrkMultiKeyring(keyringInput);
+    expect keyringRes.Success?;
+    var keyring := keyringRes.value;
     
     // This method is currently stubbed, so it doesn't matter what our input is
     var inputStructure := StructuredData(
@@ -26,7 +42,11 @@ module HappyCaseTests {
     var encryptRes := client.EncryptStructure(
       EncryptStructureInput(
         plaintextStructure:=inputStructure,
-        cryptoSchema:=schema
+        cryptoSchema:=schema,
+        keyring:=Some(keyring),
+        cmm:=None(),
+        implicitEncryptionContext:=None(),
+        explicitEncryptionContext:=None()
       )
     );
     
@@ -57,6 +77,21 @@ module HappyCaseTests {
 
   method {:test} TestDecryptStructure() {
     var client := new StructuredEncryptionClient.StructuredEncryptionClient();
+
+    // Create keyring. Currently doesn't matter what keyring we create.
+    var matProvRes := MaterialProviders.MaterialProviders(MaterialProviders.DefaultMaterialProvidersConfig());
+    expect matProvRes.Success?;
+    var matProv := matProvRes.value;
+
+    var keyringInput := AwsCryptographyMaterialProvidersTypes.CreateAwsKmsMrkMultiKeyringInput(
+        generator := Some("arn:aws:kms:us-west-2:658956600833:key/b3537ef1-d8dc-4780-9f5a-55776cbb2f7f"),
+        kmsKeyIds := None(),
+        clientSupplier := None(),
+        grantTokens := None()
+    );
+    var keyringRes := matProv.CreateAwsKmsMrkMultiKeyring(keyringInput);
+    expect keyringRes.Success?;
+    var keyring := keyringRes.value;
     
     // This method is currently stubbed, so it doesn't matter what our input is
     var inputStructure := StructuredData(
@@ -67,11 +102,17 @@ module HappyCaseTests {
       content := CryptoSchemaContent.action(CryptoAction := CryptoAction.ENCRYPT_AND_SIGN),
       attributes := None()
     );
+    var schemaMap := map[];
+    schemaMap := schemaMap["0":=schema];
 
     var encryptRes := client.DecryptStructure(
       DecryptStructureInput(
         ciphertextStructure:=inputStructure,
-        cryptoSchema:=schema
+        cryptoSchemas:=schemaMap,
+        keyring:=Some(keyring),
+        cmm:=None(),
+        implicitEncryptionContext:=None(),
+        explicitEncryptionContext:=None()
       )
     );
     
