Makefile
@@ -1,3 +1,6 @@
+ROOT_DIR:=$(shell dirname $(realpath $(firstword $(MAKEFILE_LIST))))
+DYLD_LIBRARY_PATH=$(DYLD_LIBRARY_PATH)
+
 build:
 	cd src/StructuredEncryption/src;\
 	dotnet build
@@ -9,7 +12,10 @@ test: build
 generate-models:
 	cd polymorph/smithy-dotnet;\
 	./gradlew run --args="\
-		-m src/StructuredEncryption/model\
-		-namespace aws.cryptography.structuredEncryption\
-		--output-dotnet src/StructuredEncryption/runtimes/net/Generated\
-		-d src/StructuredEncryption/model"
+	-m $(ROOT_DIR)/src/StructuredEncryption/Model \
+	-namespace aws.cryptography.structuredEncryption \
+	--output-dotnet $(ROOT_DIR)/src/StructuredEncryption/runtimes/net/Generated \
+	-d $(ROOT_DIR)/private-aws-encryption-sdk-dafny-staging/src/AwsCryptographicMaterialProviders/Model \
+	-d $(ROOT_DIR)/private-aws-encryption-sdk-dafny-staging/src/Crypto/Model \
+	-d $(ROOT_DIR)/private-aws-encryption-sdk-dafny-staging/src/AWS-KMS/Model \
+	-d $(ROOT_DIR)/private-aws-encryption-sdk-dafny-staging/model"
