README.md
@@ -8,10 +8,26 @@ Right now this repo has a bare-bones Makefile to help with some building/testing
 The Makefile doesn't currently build dev requirements, so you will need to grab these yourself.
 
 You will need at least:
-- dotnet (I'm using v5.0.402)
-- dafny (I'm using v3.4.0)
+- dotnet (I'm using v6.0.400)
+- dafny (I'm using v3.7.3)
 
 Additionally, I am working off a Mac and cannot guarantee that these commands will work on other platforms.
+
+#### System Dependencies - macOS only
+
+If you are using macOS then you must install OpenSSL 1.1,
+and the OpenSSL 1.1 `lib` directory must be on the dynamic linker path at runtime.
+We recommend that you install OpenSSL via Homebrew using `brew install openssl@1.1`,
+and then set the `DYLD_LIBRARY_PATH` environment variable as follows:
+
+```bash
+$ export DYLD_LIBRARY_PATH="/usr/local/opt/openssl@1.1/lib"
+```
+
+If the .NET runtime cannot locate your OpenSSL 1.1 libraries,
+you may encounter an error that says:
+
+> No usable version of libssl was found
 
 ### Rebuild the model
 
