src/StructuredEncryption/model/traits.smithy
@@ -1,8 +1,0 @@
-namespace aws.polymorph
-
-
-@trait(selector: "service")
-structure localService {
-    sdkId: String,
-    config: String
-}
